regular.v
@@ -1,0 +1,93 @@
+(* Decision procedures for linear integer arithmetic. *)
+
+Require Import Utf8 List.
+From larith Require Import tactics notations utilities automata.
+Import ListNotations.
+
+(* Definition of a regular predicate. *)
+Module Regularity.
+
+Section A_regular_predicate.
+
+Variable letter : Set.
+Variable P : list letter -> Prop.
+
+(* P is regular iff its domain can be decided using a DFA. *)
+Record regular := Regular {
+  r_automaton : automaton letter;
+  r_det       : Deterministic r_automaton;
+  r_size      : nat;
+  r_finite    : Finite r_automaton r_size;
+  r_dec       : ∀s t : state r_automaton, {s = t} + {s ≠ t};
+  r_spec      : ∀w, Language r_automaton w <-> P w;
+}.
+
+(* Regular predicates over a finite alphabet can be decided. *)
+Variable alphabet : list letter.
+Hypothesis full_alphabet : ∀c, In c alphabet.
+Hypothesis is_regular : regular.
+
+Theorem regular_dec :
+  {∃w, P w} + {∀w, ¬P w}.
+Proof.
+destruct is_regular as [A _ n size dec spec].
+eapply dec_replace. apply spec.
+eapply Language_inhabited_dec.
+apply full_alphabet. apply dec. apply size.
+Qed.
+
+End A_regular_predicate.
+
+Arguments regular {_}.
+
+(* Replace predicate with an equivalent one. *)
+Theorem regular_ext {letter : Set} (P Q : list letter -> Prop) :
+  regular P -> (∀w, P w <-> Q w) -> regular Q.
+Proof.
+intros [A det size fin dec spec] H.
+eapply Regular with (r_automaton:=A).
+apply det. apply fin. apply dec.
+intros; rewrite <-H; apply spec.
+Qed.
+
+(* Change the domain alphabet. *)
+Theorem regular_proj {letter letter' : Set} P Q (f : letter' -> letter) :
+  regular P -> (∀w, P (map f w) <-> Q w) -> regular Q.
+Proof.
+intros [A det size fin dec spec] H.
+pose(B := Automata.proj _ A _ (λ c, [f c])).
+eapply Regular with (r_automaton:=B).
+- apply Automata.proj_det; easy.
+- apply Automata.proj_size, fin.
+- apply dec.
+- intros. rewrite <-H, <-spec.
+  unfold B; rewrite Automata.proj_spec.
+  unfold Automata.Image; rewrite map_map_singleton. split.
+  + intros [v [H1 H2]]. apply Forall2_In_singleton in H1; congruence.
+  + intros Hfw; exists (map f w); split.
+    now apply Forall2_In_singleton. easy.
+Qed.
+
+Section Regular_operations.
+
+Variable letter : Set.
+Variable P Q : list letter -> Prop.
+
+Theorem regular_conj :
+  regular P -> regular Q -> regular (λ w, P w /\ Q w).
+Proof.
+Admitted.
+
+Theorem regular_neg :
+  regular P -> regular (λ w, ¬P w).
+Proof.
+intros [A det size fin dec spec].
+eapply Regular with (r_automaton:=Automata.compl _ A).
+apply Automata.compl_det, det. now apply Automata.compl_size, fin. apply dec.
+intros. rewrite Automata.compl_spec. split; apply contra, spec. easy.
+Qed.
+
+End Regular_operations.
+
+End Regularity.
+Export Regularity.
